LiveVerif/src/LiveVerifExamples/ErrorTests/safe_f_equal_errors.v
@@ -18,7 +18,7 @@ Goal forall n l (i j count p: word) R (m' m1 m: mem),
 Proof.
   intros. steps.
   lazymatch goal with
-  | |- don't_know_how_to_prove_equal (l[\[i]:][:\[count]]) (l[\[i]:][:\[count] + 123]) =>
+  | |- don't_know_how_to_prove eq (l[\[i]:][:\[count]]) (l[\[i]:][:\[count] + 123]) =>
       idtac
   end.
 Abort.
